coq/proof/SoundForget.v
@@ -24,6 +24,8 @@ Require InvMem.
 Require InvState.
 Require Import SoundBase.
 
+Require Import Inject. (* TODO: for simtac *)
+
 Set Implicit Arguments.
 
 Definition locals_equiv_except (ids:IdTSet.t) (locals0 locals1:GVsMap): Prop :=
@@ -46,13 +48,23 @@ Inductive state_equiv_except (ids:IdTSet.t) (st0 st1: State): Prop :=
 (*   (* unfold Forget.unary in *. *) *)
 (* Admitted. *)
 
-Lemma sem_inject_equiv_except
-      ids st0 st1 invst id val
+Lemma state_equiv_except_symm
+      ids st0 st1
+  :
+    state_equiv_except ids st0 st1 -> state_equiv_except ids st1 st0.
+Proof.
+  i. inv H. econs; eauto.
+  unfold locals_equiv_except in *.
+  symmetry. eauto.
+Qed.
+
+Lemma sem_idT_equiv_except
+      ids st0 st1 invst id gv
       (EQUIV: state_equiv_except ids st0 st1)
-      (STATE: InvState.Unary.sem_idT st0 invst id = Some val)
+      (STATE: InvState.Unary.sem_idT st0 invst id = Some gv)
       (NOTIN: ~ IdTSet.In id ids)
   :
-    <<STATE: InvState.Unary.sem_idT st1 invst id = Some val>>.
+    <<STATE: InvState.Unary.sem_idT st1 invst id = Some gv>>.
 Proof.
   unfold InvState.Unary.sem_idT in *.
   inv EQUIV.
@@ -63,17 +75,151 @@ Proof.
   symmetry. eapply LOCALS; eauto.
 Qed.
 
+Lemma sem_valueT_equiv_except
+      ids st0 st1 invst v gv
+      conf
+      (EQUIV: state_equiv_except ids st0 st1)
+      (STATE: InvState.Unary.sem_valueT conf st0 invst v = Some gv)
+      (NOTIN: (LiftPred.ValueT (flip IdTSet.mem ids)) v = false)
+  :
+    <<STATE: InvState.Unary.sem_valueT conf st1 invst v = Some gv>>.
+Proof.
+  unfold flip in NOTIN.
+  destruct v; ss.
+  eapply sem_idT_equiv_except; eauto.
+  apply IdTSetFacts.not_mem_iff; eauto.
+Qed.
+
+Lemma sem_list_valueT_equiv_except
+      ids st0 st1 invst lsv gvs
+      conf
+      (EQUIV: state_equiv_except ids st0 st1)
+      (STATE: InvState.Unary.sem_list_valueT conf st0 invst lsv = Some gvs)
+      (NOTIN: existsb (LiftPred.ValueT (flip IdTSet.mem ids) <*> snd) lsv = false)
+  :
+    <<STATE: InvState.Unary.sem_list_valueT conf st1 invst lsv = Some gvs>>.
+Proof.
+  unfold flip in NOTIN.
+  revert gvs STATE NOTIN.
+  induction lsv; ss.
+  i. simtac.
+  apply orb_false_iff in NOTIN. des.
+  exploit sem_valueT_equiv_except; eauto.
+  i.
+  des_ifs.
+(*   - ss. *)
+
+(*   destruct v; ss. *)
+(*   eapply sem_idT_equiv_except; eauto. *)
+(*   apply IdTSetFacts.not_mem_iff; eauto. *)
+(* Qed. *)
+Admitted.
+
+Ltac solve_equiv_except_val st0 :=
+  (* apply orb_false_iff in FILTER; des; *)
+  repeat match goal with
+       | [H: _ || LiftPred.ValueT _ _ = false |- _] =>
+         apply orb_false_iff in H;des
+       | [H: LiftPred.ValueT _ _ || _ = false |- _] =>
+         apply orb_false_iff in H;des
+       end;
+  repeat match goal with
+         | [H: InvState.Unary.sem_valueT _ st0 _ _ = Some _ |- _] =>
+           eapply sem_valueT_equiv_except in H; eauto; rewrite H
+         end.
+
+Lemma sem_expr_equiv_except
+      conf invst
+      ids st0 st1 e val
+      (EQUIV: state_equiv_except ids st0 st1)
+      (FILTER: (LiftPred.Expr (flip IdTSet.mem ids)) e = false)
+      (SEM_EXPR: InvState.Unary.sem_expr conf st0 invst e = Some val)
+  :
+    <<SEM_EXPR: InvState.Unary.sem_expr conf st1 invst e = Some val>>.
+Proof.
+  unfold compose in FILTER.
+  destruct e; ss; simtac;
+    try (solve_equiv_except_val st0; eauto).
+  - admit. (* lsv *)
+  - rewrite COND2. eauto.
+  - inv EQUIV. rewrite <- MEM. eauto.
+Admitted.
+
 Lemma forget_unary_sound
       ids st0 st1
-      conf invst invmem inv0 
+      conf invst invmem inv0
       (EQUIV : state_equiv_except ids st0 st1)
       (STATE : InvState.Unary.sem conf st0 invst invmem inv0)
   :
     <<STATE: InvState.Unary.sem conf st1 invst invmem (Forget.unary ids inv0)>>.
 Proof.
   inv STATE.
-  (* econs. *)
-  (* - *)
+  econs.
+  - ss.
+    ii.
+    match goal with
+    | [H: ExprPairSet.In x (ExprPairSet.filter _ _) |- _] =>
+      apply ExprPairSetFacts.filter_iff in H; [| ii; subst; eauto ]; destruct H as [IN FILTER]
+    end.
+    unfold compose, LiftPred.ExprPair in FILTER.
+    rewrite negb_orb in FILTER.
+    apply andb_true_iff in FILTER.
+    repeat rewrite negb_true_iff in FILTER. des.
+    apply state_equiv_except_symm in EQUIV.
+    exploit sem_expr_equiv_except; try exact VAL1; eauto.
+    i. des.
+    specialize (LESSDEF x IN).
+    exploit LESSDEF; eauto. i. des.
+    apply state_equiv_except_symm in EQUIV.
+    exploit sem_expr_equiv_except; try exact VAL2; eauto.
+  - ss.
+    inv NOALIAS.
+    econs.
+    + i. ss.
+      rewrite ValueTPairSetFacts.filter_b in MEM; [| ii; subst; ss].
+      des_ifs.
+      unfold compose, LiftPred.ValueTPair in MEM.
+      rewrite negb_orb in MEM. des_ifs.
+      unfold sflib.is_true in *.
+      rewrite negb_true_iff in *. ss.
+      apply state_equiv_except_symm in EQUIV.
+      exploit sem_valueT_equiv_except; try exact VAL1; eauto. i. des.
+      exploit sem_valueT_equiv_except; try exact VAL2; eauto.
+    + i. ss.
+      rewrite PtrPairSetFacts.filter_b in MEM; [| ii; subst; ss].
+      des_ifs.
+      unfold compose, LiftPred.PtrPair in MEM.
+      rewrite negb_orb in MEM. des_ifs.
+      unfold sflib.is_true in *.
+      rewrite negb_true_iff in *. ss.
+      apply state_equiv_except_symm in EQUIV.
+      unfold LiftPred.Ptr in *.
+      exploit sem_valueT_equiv_except; try exact VAL1; eauto. i. des.
+      exploit sem_valueT_equiv_except; try exact VAL2; eauto.
+  - ii. ss.
+    rewrite AtomSetFacts.filter_iff in *; [| ii; subst; ss]. des.
+    simtac.
+    rewrite <- IdTSetFacts.not_mem_iff in *.
+    exploit UNIQUE; eauto. intro SEM0.
+    inv SEM0.
+    exploit sem_idT_equiv_except; eauto.
+    { unfold InvState.Unary.sem_idT. ss. eauto. }
+    i. des.
+    econs; eauto.
+    + (* IdTSet.In (P, x) ids -> *)
+      (* lookupAL _ st1.(EC).(Locals) x = Some gv -> *)
+      (* InvState.Unary.sem_diffblock conf  *)
+      admit. (* need ids diffblock unique *)
+    + inv EQUIV.
+      rewrite <- MEM0. eauto.
+  - ii. ss.
+    unfold flip, compose in *.
+    rewrite IdTSetFacts.filter_iff in *; [| ii; subst; ss]. des.
+    simtac.
+    exploit PRIVATE; eauto.
+    eapply sem_idT_equiv_except; eauto.
+    + apply state_equiv_except_symm; eauto.
+    + apply IdTSetFacts.not_mem_iff; eauto.
 Admitted.
 
 Lemma forget_sound
@@ -94,5 +240,18 @@ Proof.
   - eapply forget_unary_sound; eauto.
   - eapply forget_unary_sound; eauto.
   - i. ss.
-    admit. (* forget maydiff *)
-Admitted.
+    unfold sflib.is_true in NOTIN.
+    apply not_true_is_false in NOTIN.
+    apply IdTSetFacts.not_mem_iff in NOTIN.
+    rewrite IdTSetFacts.union_iff in NOTIN.
+    apply not_or_and in NOTIN. des.
+    rewrite IdTSetFacts.union_iff in NOTIN.
+    apply not_or_and in NOTIN. des.
+    apply IdTSetFacts.not_mem_iff in NOTIN0.
+    ii. apply state_equiv_except_symm in EQUIV_SRC.
+    exploit sem_idT_equiv_except; try exact EQUIV_SRC; eauto. i. des.
+    exploit MAYDIFF; eauto.
+    { congruence. }
+    i. des.
+    exploit sem_idT_equiv_except; try exact EQUIV_TGT; eauto.
+Qed.
